Value.thy
@@ -26,10 +26,13 @@ lemma MaybeArithInt_None: "(MaybeArithInt f a1 a2 = None) = (\<nexists>n n'. a1 
 lemma MaybeArithInt_Not_Num: "(\<forall>n. MaybeArithInt f a1 a2 \<noteq> Some (Num n)) = (MaybeArithInt f a1 a2 = None)"
   by (metis MaybeArithInt.elims option.distinct(1))
 
+lemma MaybeArithInt_never_string: "MaybeArithInt f a b \<noteq> Some (Str x)"
+  using MaybeArithInt.elims by blast
+
 definition "value_plus = MaybeArithInt (+)"
 
-lemma plus_never_string: "MaybeArithInt f a b \<noteq> Some (Str x)"
-  using MaybeArithInt.elims by blast
+lemma value_plus_never_string: "value_plus a b \<noteq> Some (Str x)"
+  by (simp add: value_plus_def MaybeArithInt_never_string)
 
 lemma value_plus_symmetry: "value_plus x y = value_plus y x"
   apply (induct x y rule: MaybeArithInt.induct)
@@ -38,7 +41,7 @@ lemma value_plus_symmetry: "value_plus x y = value_plus y x"
 definition "value_minus = MaybeArithInt (-)"
 
 lemma minus_never_string: "value_minus a b \<noteq> Some (Str x)"
-  by (simp add: plus_never_string value_minus_def)
+  by (simp add: MaybeArithInt_never_string value_minus_def)
 
 definition "value_times = MaybeArithInt (*)"
 
