examples/Drinks_Machine.thy
@@ -80,6 +80,12 @@ lemma possible_steps_0:  "length i = 1 \<Longrightarrow> possible_steps drinks 0
   apply safe
   by (simp_all add: transitions apply_guards_def)
 
+lemma first_step_select:
+  "(s', T) |\<in>| possible_steps drinks 0 r aa b \<Longrightarrow> s' = 1 \<and> T = select"
+  apply (simp add: possible_steps_def fimage_def ffilter_def fmember_def Abs_fset_inverse Set.filter_def drinks_def)
+  apply safe
+  by (simp_all add: transitions)
+
 lemma drinks_vend_insufficient: "r $ 2 = Some (Num x1) \<Longrightarrow> x1 < 100 \<Longrightarrow> possible_steps drinks 1 r (STR ''vend'') [] = {|(1, vend_fail)|}"
   apply (simp add: possible_steps_singleton drinks_def)
   apply safe
@@ -100,19 +106,20 @@ lemma possible_steps_2_vend: "\<exists>n. r $ 2 = Some (Num n) \<and> n \<ge> 10
   by (simp_all add: transitions apply_guards_def value_gt_def join_ir_def connectives)
 
 lemma accepts_from_2: "accepts drinks 1 (<>(1 := d, 2 := Num 100)) [(STR ''vend'', [])]"
-  apply (rule accepts.step)
-  by (simp add: possible_steps_2_vend coin_def join_ir_def input2state_def value_plus_def accepts.base)
+  apply (rule accepts.step[of 2 vend])
+   apply (simp add: possible_steps_2_vend)
+  by (simp add: accepts.base)
 
 lemma accepts_from_1a: "accepts drinks 1 (<>(1 := d, 2 := Num 50)) [(STR ''coin'', [Num 50]), (STR ''vend'', [])]"
-  apply (rule accepts.step)
-  apply (simp add: possible_steps_1_coin coin_def join_ir_def input2state_def value_plus_def)
-  by (simp add: finfun_update_twist accepts_from_2)
+  apply (rule accepts.step[of 1 coin])
+   apply (simp add: possible_steps_1_coin)
+  by (simp add: coin_def join_ir_def input2state_def value_plus_def finfun_update_twist accepts_from_2)
 
 lemma accepts_from_1: "accepts drinks 1 (<>(2 := Num 0, 1 := d))
      [(STR ''coin'', [Num 50]), (STR ''coin'', [Num 50]), (STR ''vend'', [])]"
-  apply (rule accepts.step)
-  apply (simp add: possible_steps_1_coin coin_def join_ir_def input2state_def value_plus_def)
-  by (simp add: finfun_update_twist accepts_from_1a)
+  apply (rule accepts.step[of 1 coin])
+   apply (simp add: possible_steps_1_coin)
+  by (simp add: coin_def join_ir_def input2state_def value_plus_def finfun_update_twist accepts_from_1a)
 
 lemma purchase_coke: "observe_trace drinks 0 <> [(STR ''select'', [Str ''coke'']), (STR ''coin'', [Num 50]), (STR ''coin'', [Num 50]), (STR ''vend'', [])] =
                        [[], [Some (Num 50)], [Some (Num 100)], [Some (Str ''coke'')]]"
@@ -138,7 +145,7 @@ lemma purchase_coke: "observe_trace drinks 0 <> [(STR ''select'', [Str ''coke'']
   by simp
 
 lemma rejects_input: "l \<noteq> STR ''coin'' \<Longrightarrow> l \<noteq> STR ''vend'' \<Longrightarrow> \<not> accepts drinks 1 d' [(l, i)]"
-  apply (rule trace_reject_no_possible_steps)
+  apply (rule no_possible_steps_rejects)
   by (simp add: possible_steps_empty drinks_def can_take_transition_def can_take_def transitions)
 
 lemma rejects_accepts_prefix:
@@ -194,7 +201,7 @@ lemma drinks_1_rejects: "fst a = STR ''coin'' \<longrightarrow> length (snd a) \
   by (metis decompose_pair)
 
 lemma drinks_rejects_future: "rejects drinks 2 d ((l, i)#t)"
-  apply (rule trace_reject_no_possible_steps)
+  apply (rule no_possible_steps_rejects)
   by (simp add: possible_steps_empty drinks_def)
 
 lemma drinks_1_rejects_trace:
@@ -216,7 +223,11 @@ lemma rejects_state_step: "s > 1 \<Longrightarrow> step drinks s r l i = None"
   by (simp add: possible_steps_empty drinks_def)
 
 lemma invalid_other_states: "s > 1 \<Longrightarrow> rejects drinks s r ((aa, b) # t)"
-  apply (rule trace_reject_no_possible_steps)
+  apply (rule no_possible_steps_rejects)
   by (simp add: possible_steps_empty drinks_def)
+
+lemma vend_ge_100: "possible_steps drinks 1 r l i = {|(2, vend)|} \<Longrightarrow> \<not>\<^sub>? value_gt (Some (Num 100)) (r $ 2) = trilean.true"
+  apply (insert possible_steps_apply_guards[of drinks 1 r l i 2 vend])
+  by (simp add: possible_steps_def apply_guards_def vend_def)
 
 end
